case_study/RiscvPmp/LoopVerification.v
@@ -60,9 +60,10 @@ Import ListNotations.
 Import RiscvPmpSpecification.
 Import RiscvPmpProgram.
 Import RiscvPmpIrisBase.
-Import RiscvPmpIrisInstance.
 Import RiscvPmpModel2.
+Import RiscvPmpModel2.RiscvPmpIrisInstance.
 Import RiscvPmpValidContracts.
+Import RiscvPmpIrisInstancePredicates.
 
 Import RiscvPmpSignature.
 Module Import RiscvPmpShallowExecutor :=
@@ -320,7 +321,7 @@ Section Loop.
   Proof.
     iApply (@iris_rule_consequence _ _ _ _ env.nil
              ((∃ p : Privilege, cur_privilege ↦ p) ∗
-              (∃ es : list RiscvPmpIrisInstance.PmpEntryCfg, interp_pmp_entries es))
+              (∃ es : list PmpEntryCfg, interp_pmp_entries es))
              _ _ _ fun_init_model _ _).
     iApply valid_init_model_contract.
     Unshelve.
